### 第三章习题（基本）

郑盛东 2024213760

#### 3.1 

$G(x)=x+2^{3} x^{2}+3^{3} x^{3}+\ldots=\sum_{n=0}^{\infty} n^{3} x^{n}$

设$e(x)=\frac{1}{1-x}=\sum_{n=0}^{\infty}  x^{n}$

由求导性质，$\sum_{n=0}^{\infty} n x^{n}=x e^{(1)}(x)=\frac{x}{(1-x)^{2}}$

设$f(x)=\frac{x}{(1-x)^{2}}=\sum_{n=0}^{\infty} n x^{n}$

由求导性质，$\sum_{n=0}^{\infty} n^{2} x^{n}=x f^{(1)}(x)=\frac{x}{(1-x)^{2}}+\frac{2x^{2}}{(1-x)^3}$

设$g(x) = \frac{x}{(1-x)^{2}}+\frac{2x^{2}}{(1-x)^3}=\sum_{n=0}^{\infty} n^{2} x^{n}$

由求导性质，$\sum_{n=0}^{\infty} n^{3} x^{n}=x g^{(1)}(x)=\frac{x}{(1-x)^2} + \frac{6x^2}{(1-x)^3} + \frac{6x^3}{(1-x)^4}$

所以$G(x)=\sum_{n=0}^{\infty} n^{3} x^{n}=\frac{x}{(1-x)^2} + \frac{6x^2}{(1-x)^3} + \frac{6x^3}{(1-x)^4}$

#### 3.2 

$G(x)=\sum_{n=0}^{\infty} \binom{n+3}{3} x^{n}=\sum_{n=0}^{\infty} \frac{(n+3)(n+2)(n+1)}{6}x^{n}$

设$e(x)=\sum_{n=0}^{\infty}x^{n+3}=\frac{x^3}{1-x}=-x^2-x-1+\frac{1}{1-x}$

由求导性质，$\sum_{n=0}^{\infty} (n+3) x^{n+2}=e^{(1)}(x)$

同理可得，$\sum_{n=0}^{\infty} (n+3)(n+2)(n+1) x^{n}=e^{(3)}(x)=\frac{6}{(1-x)^{4}}$

所以$G(x)=\sum_{n=0}^{\infty} \binom{n+3}{3} x^{n}=\sum_{n=0}^{\infty} \frac{(n+3)(n+2)(n+1)}{6}x^{n}=\frac{1}{(1-x)^{4}}$

#### 3.3  

根据定义，$a_0=1,a_1=1^3+2^3,\ldots,a_n=1^3+2^3+\ldots+(n+1)^3$

$G(x)=1^3+(1^3+2^3)x+(1^3+2^3+3^3)x^2+\ldots+(1^3+2^3+\ldots+(n+1)^3)x^n \\ =1^3(1+x+\ldots)+2^3(x+x^2+\ldots)+\ldots+(n+1)^3(x^n+x^{n+1}+\ldots)\\=\frac{1^3}{1-x}+\frac{2^3x}{1-x}+\ldots\\=\frac{1}{1-x}\sum_{n=0}^{\infty}(n+1)^3x^n$

设3.1的母函数为A(x)，由母函数性质$G(x)=\frac{1}{1-x}\frac{A(x)}{x}=\frac{1}{(1-x)^3} + \frac{6x}{(1-x)^4} + \frac{6x^2}{(1-x)^5}$

#### 3.4

根据{bn}定义，$\sum_{i=0}^{n}b_i=a_n$，由母函数定义，$A(x)=\frac{B(x)}{1-x}$

所以，$B(x)=(1-x)A(x)=\frac{4-3x}{1+x-x^3}$



