# 第三章作业-基本
## 2024213751 姜华祖

### 3.1
* 母函数 \( G(x) \) 定义为：

\[
G(x) = \sum_{n=0}^\infty a_n x^n = \sum_{n=0}^\infty n^3 x^n
\]
* 已知：
\[
   \sum_{n=0}^\infty x^n = \frac{1}{1 - x}
\]
* 两边求导：
\[
   \sum_{n=0}^\infty n x^{n-1} = \frac{1}{(1 - x)^2} \implies \sum_{n=0}^\infty n x^n = \frac{x}{(1 - x)^2}
\]

* 两边求导：

   \[
   \frac{d}{dx} \left( \frac{x}{(1 - x)^2} \right ) = \frac{(1 - x)^2 + 2x(1 - x)}{(1 - x)^4} = \frac{1 + x}{(1 - x)^3}
   \]

   \[
   \sum_{n=0}^\infty n^2 x^n = \frac{x(1 + x)}{(1 - x)^3}
   \]

* 两边求导：

\[
   \frac{d}{dx} \left( \frac{x(1 + x)}{(1 - x)^3} \right ) = \frac{(1 + 2x)(1 - x)^3 + 3x(1 + x)(1 - x)^2}{(1 - x)^6}
\]
   
\[
   \sum_{n=0}^\infty n^3 x^n = \frac{x(x^2 + 4x + 1)}{(1 - x)^4}
\]

* 所以，数列 \(\{ a_n \}\) 的母函数为：

\[
G(x) = \sum_{n=0}^\infty n^3 x^n = \frac{x(x^2 + 4x + 1)}{(1 - x)^4}
\]
### 3.2


\[
a_n = \binom{n+3}{3} = \frac{(n+3)(n+2)(n+1)}{6}
\]

* 已知：

\[
\sum_{n=0}^{\infty} x^n = \frac{1}{1 - x}
\]

* 两边求导：
\[
\sum_{n=1}^{\infty} n x^{n-1} = \frac{1}{(1 - x)^2}
\]

* 两边求导：

\[
\sum_{n=2}^{\infty} n(n-1) x^{n-2} = \frac{2}{(1 - x)^3}
\]

* 两边求导

\[
\sum_{n=3}^{\infty} n(n-1)(n-2) x^{n-3} = \frac{6}{(1 - x)^4}
\]



* 统一下标：

\[
\sum_{n=0}^{\infty} (n+3)(n+2)(n+1) x^n = \frac{6}{(1 - x)^4}
\]

\[
G(x) = \sum_{n=0}^{\infty} a_n x^n = \frac{1}{(1 - x)^4}
\]
\[
G(x) = \frac{1}{(1 - x)^4}
\]

### 3.3
* 将3.1的母函数和\(\frac{1}{1-x}\)相乘即可。
\[
G(x) = \frac{x(x^2 + 4x + 1)}{(1 - x)^5}
\]

### 3.4
\[
B(x) = \sum_{n=0}^{\infty} b_n x^n = b_0 + \sum_{n=1}^{\infty} (a_n - a_{n-1}) x^n
\]
\[
B(x) = a_0 + (A(x) - a_0) - x A(x) = A(x) - x A(x) = A(x)(1 - x)
\]
\[
B(x) = \frac{4-3x}{1+x-x^3}
\]