# hw3 基本

## 3.1

$$
\begin{align}
\sum x^n &= \frac{1}{1 - x} \\
\sum nx^n &= x \cdot \frac{\mathrm d}{\mathrm dx} (\sum x^n) = x \cdot \frac{\mathrm d}{\mathrm dx} (\frac{1}{1-x}) = \frac{x}{(1 - x)^2} \\
\sum n^2 x^n &= x \cdot \frac{\mathrm d}{\mathrm dx} (\sum n x^n) = x \cdot \frac{\mathrm d}{\mathrm dx} (\frac{x}{(1 - x)^2}) = \frac{x(1 + x)}{(1 - x)^3} \\
\sum n^3 x^n &= x \cdot \frac{\mathrm d}{\mathrm dx} (\sum n^2 x^n) = x \cdot \frac{\mathrm d}{\mathrm dx}(\frac{x(1 + x)}{(1 - x)^3}) = x \frac{1 + 4x + x^2}{(1 - x)^4}
\end{align}
$$



## 3.2

$$
\begin{align}
\sum a_n x^n &= \sum \dbinom{n + 3}{3} x^n = \frac{(n + 3)(n + 2)(n + 1)}{6} x^n \\
&= \frac 1 6\sum (n^3 + 6n^2 + 11n + 6) x^n \\
&= \frac 1 6 [\sum n^3 x^n + 6 \sum n^2 x^n + 11 \sum nx^n + 6 \sum x^n] \\
&= \frac 1 6 [\frac{x(1 + 4x + x^2)}{(1 - x)^4} + \frac{6x(1 + x)}{(1 - x)^3} + \frac{11x}{(1 - x)^2} + \frac{6}{1 - x}] \\
&= \frac{1}{(1 - x)^4}
\end{align}
$$



## 3.3

$$
\because \sum n^3 x^n = x \frac{1 + 4x + x^2}{(1 - x)^4} \\
\therefore \sum (n + 1)^3 x^n = \frac{1}{x} (\sum n^3 x^n) = \frac{1 + 4x + x^2}{(1 - x)^4} \\
\therefore \sum (\sum \limits_{k = 1}^{n + 1} k^3) x^n = (1 + x + x^2 + x^3 + \dots) \sum (n + 1)^3 x^n \\
= \frac{1}{1 - x} \frac{1 + 4x + x^2}{(1 - x)^4} = \frac{1 + 4x + x^2}{(1 - x)^5}
$$





## 3.4

$$
\begin{align}
A(x) &= a_0 + a_1x + a_2x^2 + a_3 x^3 + \dots \\
xA(x) &= 0 + a_0x + a_1x^2 + a_2x^3 + \dots \\
(1 - x)A(x) &= a_0 + (a_1 - a_0) x + (a_2 - a_1) x^2 + (a_3 - a_2) x^3 \\
&= \sum b_n x^n \\
&= (1 - x)A(x) = \frac{4 - 3x}{1 + x - x^3}
\end{align}
$$

