3.1

$$A(x) = \sum_{n=0}^{\infty} n^3 x^n$$

已知：$\sum_{n=0}^{\infty} x^n = \frac{1}{1-x}$ ，求导有 $\sum_{n=0}^{\infty} n x^{n-1} = \frac{1}{(1-x)^2}$ ，进一步乘x有 $\sum_{n=0}^{\infty} n x^{n}= \frac{x}{(1-x)^2}$  ，进一步求导： $\sum_{n=0}^{\infty} n^2 x^{n-1} = \frac{x+1}{(1-x)^3}$ ，从而 $\sum_{n=0}^{\infty} n^2 x^{n} = \frac{x^2+x}{(1-x)^3}$ ；进一步求导：$\sum_{n=0}^{\infty} n^3 x^{n-1} = \frac{x^2+4x+1}{(1-x)^4}$ ，进而$\sum_{n=0}^{\infty} n^3 x^{n} = \frac{x^3+4x^2+x}{(1-x)^4}$ 

所以，$A(x)  = \frac{x^3+4x^2+x}{(1-x)^4}$



3.2

$A(x) = \sum_{n=0}^{\infty} (_3^{n+3}) x^n = \frac16 (\sum_{n=0}^{\infty} (n^3+6n^2+11n+6)x^n) = \frac16(\frac{x^3+4x^2+x}{(1-x)^4} + 6\frac{x^2+x}{(1-x)^3} + 11 \frac x{(1-x)^2}+\frac 6 {1-x}) = \frac 1 {(1-x)^4}$

 

3.3

$$A(x)  = \sum_{n=0}^{\infty} (\sum_{k=1}^{n+1} k^3) x^n \\ = 1^3 + (1^3+2^3)x+(1^3+2^3+3^3)x^2+(1^3+2^3+3^3+4^3)x^3+\cdots \\ =1^3+1^3(x+x^2+x^3+\cdots)+2^3(x+x^2+x^3+\cdots)+3^3(x^2+x^3+\cdots) \\ =1^3(1+x+x^2+x^3+\cdots)+2^3x(1+x+x^2+\cdots)+3^3x^2(1+x+\cdots) = (1^3+2^3x+3^3x^2+4^3x^3)\frac{1}{1-x} = \frac{x^3+4x^2+x}{(1-x)^5}$$ 

3.4

$$B(x) = \sum_{n=0}^{\infty} b_n x^n = a_0 + \sum_{n=1}^\infty (a_n - a_{n-1}) x^n = \sum_{n=0}^{\infty} a_n x^n - \sum_{n=0}^{\infty} a_n x^{n+1}\\ = A(x)-xA(x) = \frac{4-3x}{(1-x)(1+x-x^3)} - \frac{4x-3x^2}{(1-x)(1+x-x^3)}=\frac{3x-4}{x^3-x-1}$$

